isabelle/PositiveAccounts.thy
@@ -19,6 +19,12 @@ lemma addMoneyToAccountPositive_noMatch :
   apply simp
   by (simp add: insert_lookup_different)
 
+lemma updateMoneyInAccount_geZero :
+ "0 < newBalance \<Longrightarrow>
+  \<forall>x. 0 \<le> moneyInAccount x accs \<Longrightarrow>
+  0 \<le> moneyInAccount y (updateMoneyInAccount accId newBalance accs)"
+  by (metis addMoneyToAccountPositive_noMatch addMoneyToAccountPositve_match not_less updateMoneyInAccount.simps)
+
 lemma addMoneyToAccountPositive :
   "0 \<le> money \<Longrightarrow> (\<forall>x. moneyInAccount x accs \<ge> 0)
   \<Longrightarrow> moneyInAccount y (addMoneyToAccount accId money accs) \<ge> 0"
@@ -27,19 +33,88 @@ lemma addMoneyToAccountPositive :
   apply simp
   apply (simp del:moneyInAccount.simps)
   apply (cases "accId = y")
-  apply (metis (full_types) addMoneyToAccountPositve_match add_le_same_cancel1 dual_order.trans not_less)
-proof -
-  assume a1: "accId \<noteq> y"
-assume a2: "\<not> money \<le> 0"
-  assume a3: "\<forall>x. 0 \<le> moneyInAccount x accs"
-  then have f4: "\<not> moneyInAccount accId accs + money \<le> 0"
-using a2 by (meson add_le_same_cancel1 le_less_trans not_less)
-  have "\<And>i. \<not> 0 < i \<or> 0 \<le> moneyInAccount y (MList.insert accId i accs)"
-    using a3 a1 addMoneyToAccountPositive_noMatch by blast
-then show "0 \<le> moneyInAccount y (let i = moneyInAccount accId accs + money in if i \<le> 0 then MList.delete accId accs else MList.insert accId i accs)"
-  using f4 by auto
-qed
+  apply (smt updateMoneyInAccount.simps updateMoneyInAccount_geZero)
+  by (smt updateMoneyInAccount.simps updateMoneyInAccount_geZero)
 
+lemma giveMoney_geZero :
+    "\<forall>x. 0 \<le> moneyInAccount x accs \<Longrightarrow>
+       (eff, newAccs) = giveMoney payee money accs \<Longrightarrow> 
+       0 \<le> moneyInAccount y newAccs"
+  by (metis addMoneyToAccount.simps addMoneyToAccountPositive giveMoney.elims linear snd_conv)
+
+lemma moneyInAccount_valid_zero : "valid_map ((accId, money) # rest) \<Longrightarrow> moneyInAccount accId rest = 0"
+  apply (simp only:moneyInAccount.simps findWithDefault.simps)
+  by (simp add: MList.delete_lookup_None_aux)
+
+lemma moneyInAccount_sublist_geZero_different :
+  "valid_map ((accId, money) # rest) \<Longrightarrow>
+   0 < money \<Longrightarrow> 0 \<le> moneyInAccount y ((accId, money) # rest) \<Longrightarrow>
+   accId \<noteq> y \<Longrightarrow> 0 \<le> moneyInAccount y rest"
+  apply (simp only:moneyInAccount.simps findWithDefault.simps)
+  by (metis MList.delete.simps(2) MList.different_delete_lookup)
+
+lemma moneyInAccount_sublist_geZero :
+    "valid_map ((accId, money) # rest) \<Longrightarrow>
+     money > 0 \<Longrightarrow>
+    (\<forall>x. 0 \<le> moneyInAccount x ((accId, money) # rest)) \<Longrightarrow> 0 \<le> moneyInAccount y rest"
+  apply (cases "accId = y")
+  using moneyInAccount_valid_zero apply auto[1]
+  using moneyInAccount_sublist_geZero_different by blast
+
+lemma moneyInAccount_geZero_preservation :
+  "valid_map ((accId, money) # rest) \<Longrightarrow>
+   (\<forall>x. 0 \<le> moneyInAccount x ((accId, money) # rest)) \<Longrightarrow> 0 \<le> moneyInAccount y rest"
+  apply (simp only:moneyInAccount.simps findWithDefault.simps)
+  by (metis MList.delete.simps(2) MList.delete_lookup_None_aux MList.delete_valid_aux MList.insert_in_middle lookup.simps(2) not_less_iff_gr_or_eq option.simps(4) order_refl)
+
+lemma reduceOne_geZero_aux :
+  "valid_map ((accId, money) # rest) \<Longrightarrow>
+   (money \<le> 0 \<Longrightarrow> \<forall>x. 0 \<le> moneyInAccount x rest \<Longrightarrow> refundOne rest = Some (paym, newAccs) \<Longrightarrow> 0 \<le> moneyInAccount y newAccs) \<Longrightarrow>
+   \<forall>x. 0 \<le> moneyInAccount x ((accId, money) # rest) \<Longrightarrow> refundOne ((accId, money) # rest) = Some (paym, newAccs) \<Longrightarrow> 0 \<le> moneyInAccount y newAccs"
+  apply (cases "money > 0")
+  apply (simp only:refundOne.simps)
+  using moneyInAccount_sublist_geZero apply auto[1]
+  apply (simp only:refundOne.simps if_False)
+  using moneyInAccount_geZero_preservation not_less by blast
+
+lemma reduceOne_geZero :
+  "valid_map accs \<Longrightarrow>
+   \<forall>x. 0 \<le> moneyInAccount x accs \<Longrightarrow>
+   refundOne accs = Some (paym, newAccs) \<Longrightarrow>
+   0 \<le> moneyInAccount y newAccs"
+  apply (induction accs rule:"refundOne.induct")
+  apply (meson MList.sublist_valid not_le reduceOne_geZero_aux)
+  by auto
+
+lemma reduceContractStep_geZero_Refund_aux : 
+  "valid_state state \<Longrightarrow>
+   \<forall>x. 0 \<le> moneyInAccount x (accounts state) \<Longrightarrow>
+   refundOne (accounts state) = Some ((party, money), newAccount) \<Longrightarrow>
+   wa = ReduceNoWarning \<Longrightarrow>
+   eff = ReduceWithPayment (Payment party money) \<Longrightarrow>
+   0 \<le> moneyInAccount y newAccount"
+  using reduceOne_geZero valid_state.elims(2) by blast
+
+lemma reduceContractStep_geZero_Refund : 
+  "valid_state state \<Longrightarrow>
+   \<forall>x. 0 \<le> moneyInAccount x (accounts state) \<Longrightarrow>
+   refundOne (accounts state) = Some ((party, money), newAccount) \<Longrightarrow> 
+   Reduced ReduceNoWarning (ReduceWithPayment (Payment party money)) (state\<lparr>accounts := newAccount\<rparr>) Refund =
+      Reduced wa eff newState newCont \<Longrightarrow>
+   0 \<le> moneyInAccount y (accounts newState)"
+  using reduceContractStep_geZero_Refund_aux by auto
+
+lemma reduceContractStep_geZero :
+  "valid_state state \<Longrightarrow>
+   (\<forall>x. moneyInAccount x (accounts state) \<ge> 0) \<Longrightarrow>
+   reduceContractStep env state cont = Reduced wa eff newState newCont \<Longrightarrow>
+   moneyInAccount y (accounts newState) \<ge> 0"
+  apply (cases cont)
+  apply (simp only:reduceContractStep.simps)
+  apply (cases "refundOne (accounts state)")
+  apply simp
+  using reduceContractStep_geZero_Refund apply force
+  oops
 
 (* Alternative formulation *)
 
@@ -58,6 +133,11 @@ lemma addMoneyToAccountPositive :
   \<Longrightarrow> allAccountsPositive (addMoneyToAccount accId money accs)"
   oops
 
+theorem accountsArePositive :
+"(\<forall>x. moneyInAccount x (accounts state) \<ge> 0) \<Longrightarrow>
+  computeTransaction txIn state cont = TransactionOutput txOut \<Longrightarrow>
+  moneyInAccount y (accounts (txOutState txOut)) \<ge> 0"
+oops
 
 theorem accountsArePositive2 :
     "allAccountsPositiveState state
